01Expression/Typecheck.thy
@@ -269,4 +269,72 @@ lemma tc_weaken [simp]: "\<Delta>,\<Gamma> \<turnstile> e : t \<Longrightarrow> 
     ultimately show ?case by fastforce
   qed fastforce+
 
+lemma tc_free_var: "lookup x (\<Gamma>' @ \<Gamma>) = Some t \<Longrightarrow> x \<notin> (\<lambda>x. length \<Gamma>' + x) ` {x. x < length \<Gamma>} \<Longrightarrow> 
+    lookup x \<Gamma>' = Some t"
+  proof (induction "x < length \<Gamma>'")
+  case False
+    moreover then obtain y where "x = length \<Gamma>' + y" by fastforce
+    ultimately show ?thesis by fastforce
+  qed simp_all
+
+lemma tc_freevars_xs: "\<Delta> ,\<Gamma>'@\<Gamma> \<turnstile>\<^sub>x\<^sub>s xs : ts \<Longrightarrow> 
+    set xs \<inter> (\<lambda>x. length \<Gamma>' + x) ` {x. x < length \<Gamma>} = {} \<Longrightarrow> \<Delta>,\<Gamma>' \<turnstile>\<^sub>x\<^sub>s xs : ts"
+  proof (induction \<Delta> "\<Gamma>'@\<Gamma>" xs ts rule: typecheck_xs.induct) 
+  case tcx_cons
+    thus ?case using tc_free_var by force
+  qed simp_all
+
+lemma [simp]: "var_reduce xs \<inter> (op +) n ` ys = {} \<Longrightarrow> xs \<inter> (op +) (Suc n) ` ys = {}"
+  proof -
+    assume R: "var_reduce xs \<inter> (op +) n ` ys = {}"
+    have "\<And>x. x \<in> xs \<Longrightarrow> x \<notin> (op +) (Suc n) ` ys" 
+      proof 
+        fix x
+        assume XS: "x \<in> xs"
+        assume YS: "x \<in> (op +) (Suc n) ` ys"
+        thus False 
+          proof (cases x)
+          case (Suc x')
+            with XS have "x' \<in> (\<lambda>x. x - 1) ` (xs - {0})" by force
+            with R YS Suc show False by (auto simp add: var_reduce_def)
+          qed auto
+      qed
+    thus "xs \<inter> (op +) (Suc n) ` ys = {}" by auto
+  qed
+
+lemma tc_freevars: "\<Delta>,\<Gamma>'@\<Gamma> \<turnstile> e : t \<Longrightarrow> 
+    free_vars e \<inter> (\<lambda>x. length \<Gamma>' + x) ` {x. x < length \<Gamma>} = {} \<Longrightarrow> \<Delta>,\<Gamma>' \<turnstile> e : t"
+  and "\<Delta>,\<Gamma>'@\<Gamma> \<turnstile>\<^sub>c cs : ts \<rightarrow> t \<Longrightarrow> free_vars\<^sub>c cs \<inter> (\<lambda>x. length \<Gamma>' + x) ` {x. x < length \<Gamma>} = {} \<Longrightarrow> 
+    \<Delta>,\<Gamma>' \<turnstile>\<^sub>c cs : ts \<rightarrow> t "
+  proof (induction \<Delta> "\<Gamma>'@\<Gamma>" e t and \<Delta> "\<Gamma>'@\<Gamma>" cs ts t arbitrary: \<Gamma>' \<Gamma> and \<Gamma>' \<Gamma>
+         rule: typecheck_typecheck_cs.inducts)
+  case tc_var
+    thus ?case using tc_free_var by fastforce
+  next case (tc_let \<Delta> e\<^sub>1 t\<^sub>1 e\<^sub>2 t\<^sub>2)
+    moreover hence "var_reduce (free_vars e\<^sub>2) \<inter> op + (length \<Gamma>') ` {x. x < length \<Gamma>} = {}" by auto
+    ultimately have "\<Delta>,insert_at 0 t\<^sub>1 \<Gamma>' \<turnstile> e\<^sub>2 : t\<^sub>2" by simp
+    moreover from tc_let have "\<Delta>,\<Gamma>' \<turnstile> e\<^sub>1 : t\<^sub>1" by fastforce
+    ultimately show ?case by simp
+  next case tc_rec
+    thus ?case using tc_freevars_xs by fastforce
+  next case tc_inj
+    thus ?case using tc_free_var by fastforce
+  next case tc_fold
+    thus ?case using tc_free_var by fastforce
+  next case (tcc_cons \<Delta> t' e t cs ts)
+    moreover hence "var_reduce (free_vars e) \<inter> op + (length \<Gamma>') ` {x. x < length \<Gamma>} = {}" by auto
+    ultimately have "\<Delta>,insert_at 0 t' \<Gamma>' \<turnstile> e : t" by simp
+    moreover from tcc_cons have "\<Delta>,\<Gamma>' \<turnstile>\<^sub>c cs : ts \<rightarrow> t" by fastforce
+    ultimately show ?case by simp
+  qed fastforce+
+
+lemma [simp]: "\<Delta>,\<Gamma> \<turnstile> e : t \<Longrightarrow> free_vars e \<inter> {x. x < length \<Gamma>} = {} \<Longrightarrow> \<Delta>,[] \<turnstile> e : t"
+  proof -
+    assume "\<Delta>,\<Gamma> \<turnstile> e : t"
+    hence X: "\<Delta>,[]@\<Gamma> \<turnstile> e : t" by simp
+    assume "free_vars e \<inter> {x. x < length \<Gamma>} = {}"
+    hence "free_vars e \<inter> (\<lambda>x. length [] + x) ` {x. x < length \<Gamma>} = {}" by simp
+    with X show "\<Delta>,[] \<turnstile> e : t" by (metis tc_freevars)
+  qed
+ 
 end
