Utilities/Index.thy
@@ -8,10 +8,6 @@ definition incr :: "nat \<Rightarrow> nat \<Rightarrow> nat" where
 definition decr :: "nat \<Rightarrow> nat \<Rightarrow> nat" where
   "decr x y = (if x < y then y - 1 else y)"
 
-primrec zero_to :: "nat \<Rightarrow> nat set" where
-  "zero_to 0 = {}"
-| "zero_to (Suc x) = insert x (zero_to x)"
-
 lemma [simp]: "lookup y as = Some a \<Longrightarrow> x \<le> length as \<Longrightarrow> 
     lookup (incr x y) (insert_at x a' as) = Some a"
   by (simp add: incr_def)
@@ -20,7 +16,10 @@ lemma [simp]: "lookup y (insert_at x a' as) = Some a \<Longrightarrow> x \<le> l
     lookup x' as = Some a' \<Longrightarrow> x \<noteq> y \<Longrightarrow> lookup (decr x y) as = Some a"
   by (cases y) (auto simp add: decr_def)
 
-lemma [elim]: "zero_to x = {} \<Longrightarrow> x = 0"
-  by (induction x) simp_all
+lemma [simp]: "(x::nat) \<ge> y \<Longrightarrow> \<exists>z. x = y + z"
+  proof (induction x arbitrary: y)
+  case Suc
+    thus ?case by (induction y) simp_all
+  qed simp_all
 
 end
